theories/examples/syntax/syntax.v
@@ -15,7 +15,13 @@ Inductive Tm (n_Tm : nat) : Type :=
   | tnat : Tm n_Tm
   | tpi : Tm n_Tm -> Tm (S n_Tm) -> Tm n_Tm
   | tuniv : Tm n_Tm
-  | fix_ : Tm n_Tm -> Tm n_Tm.
+  | fix_ : Tm n_Tm -> Tm n_Tm
+  (* Identity fragment (Agda [ID/Syntax/Raw.agda]).  All three are binder-free:
+     the motive [C] and base [d] of [jcase] are ordinary terms of the derived
+     Pi-types [motive_ty A] / [base_ty A C]. *)
+  | tid : Tm n_Tm -> Tm n_Tm -> Tm n_Tm -> Tm n_Tm
+  | rfl : Tm n_Tm -> Tm n_Tm
+  | jcase : Tm n_Tm -> Tm n_Tm -> Tm n_Tm -> Tm n_Tm.
 
 Lemma congr_abs {m_Tm : nat} {s0 : Tm m_Tm} {s1 : Tm (S m_Tm)} {t0 : Tm m_Tm}
   {t1 : Tm (S m_Tm)} (H0 : s0 = t0) (H1 : s1 = t1) :
@@ -79,6 +85,32 @@ Proof.
 exact (eq_trans eq_refl (ap (fun x => fix_ m_Tm x) H0)).
 Qed.
 
+Lemma congr_tid {m_Tm : nat} {s0 : Tm m_Tm} {s1 : Tm m_Tm} {s2 : Tm m_Tm}
+  {t0 : Tm m_Tm} {t1 : Tm m_Tm} {t2 : Tm m_Tm} (H0 : s0 = t0) (H1 : s1 = t1)
+  (H2 : s2 = t2) : tid m_Tm s0 s1 s2 = tid m_Tm t0 t1 t2.
+Proof.
+exact (eq_trans
+         (eq_trans (eq_trans eq_refl (ap (fun x => tid m_Tm x s1 s2) H0))
+            (ap (fun x => tid m_Tm t0 x s2) H1))
+         (ap (fun x => tid m_Tm t0 t1 x) H2)).
+Qed.
+
+Lemma congr_rfl {m_Tm : nat} {s0 : Tm m_Tm} {t0 : Tm m_Tm} (H0 : s0 = t0) :
+  rfl m_Tm s0 = rfl m_Tm t0.
+Proof.
+exact (eq_trans eq_refl (ap (fun x => rfl m_Tm x) H0)).
+Qed.
+
+Lemma congr_jcase {m_Tm : nat} {s0 : Tm m_Tm} {s1 : Tm m_Tm} {s2 : Tm m_Tm}
+  {t0 : Tm m_Tm} {t1 : Tm m_Tm} {t2 : Tm m_Tm} (H0 : s0 = t0) (H1 : s1 = t1)
+  (H2 : s2 = t2) : jcase m_Tm s0 s1 s2 = jcase m_Tm t0 t1 t2.
+Proof.
+exact (eq_trans
+         (eq_trans (eq_trans eq_refl (ap (fun x => jcase m_Tm x s1 s2) H0))
+            (ap (fun x => jcase m_Tm t0 x s2) H1))
+         (ap (fun x => jcase m_Tm t0 t1 x) H2)).
+Qed.
+
 Lemma upRen_Tm_Tm {m : nat} {n : nat} (xi : fin m -> fin n) :
   fin (S m) -> fin (S n).
 Proof.
@@ -106,6 +138,12 @@ Fixpoint ren_Tm {m_Tm : nat} {n_Tm : nat} (xi_Tm : fin m_Tm -> fin n_Tm)
   | tpi _ s0 s1 => tpi n_Tm (ren_Tm xi_Tm s0) (ren_Tm (upRen_Tm_Tm xi_Tm) s1)
   | tuniv _ => tuniv n_Tm
   | fix_ _ s0 => fix_ n_Tm (ren_Tm xi_Tm s0)
+  | tid _ s0 s1 s2 =>
+      tid n_Tm (ren_Tm xi_Tm s0) (ren_Tm xi_Tm s1) (ren_Tm xi_Tm s2)
+  | rfl _ s0 =>
+      rfl n_Tm (ren_Tm xi_Tm s0)
+  | jcase _ s0 s1 s2 =>
+      jcase n_Tm (ren_Tm xi_Tm s0) (ren_Tm xi_Tm s1) (ren_Tm xi_Tm s2)
   end.
 
 Lemma up_Tm_Tm {m : nat} {n_Tm : nat} (sigma : fin m -> Tm n_Tm) :
@@ -138,6 +176,12 @@ Fixpoint subst_Tm {m_Tm : nat} {n_Tm : nat} (sigma_Tm : fin m_Tm -> Tm n_Tm)
       tpi n_Tm (subst_Tm sigma_Tm s0) (subst_Tm (up_Tm_Tm sigma_Tm) s1)
   | tuniv _ => tuniv n_Tm
   | fix_ _ s0 => fix_ n_Tm (subst_Tm sigma_Tm s0)
+  | tid _ s0 s1 s2 =>
+      tid n_Tm (subst_Tm sigma_Tm s0) (subst_Tm sigma_Tm s1) (subst_Tm sigma_Tm s2)
+  | rfl _ s0 =>
+      rfl n_Tm (subst_Tm sigma_Tm s0)
+  | jcase _ s0 s1 s2 =>
+      jcase n_Tm (subst_Tm sigma_Tm s0) (subst_Tm sigma_Tm s1) (subst_Tm sigma_Tm s2)
   end.
 
 Lemma upId_Tm_Tm {m_Tm : nat} (sigma : fin m_Tm -> Tm m_Tm)
@@ -182,6 +226,12 @@ subst_Tm sigma_Tm s = s :=
         (idSubst_Tm (up_Tm_Tm sigma_Tm) (upId_Tm_Tm _ Eq_Tm) s1)
   | tuniv _ => congr_tuniv
   | fix_ _ s0 => congr_fix_ (idSubst_Tm sigma_Tm Eq_Tm s0)
+  | tid _ s0 s1 s2 =>
+      congr_tid (idSubst_Tm sigma_Tm Eq_Tm s0) (idSubst_Tm sigma_Tm Eq_Tm s1) (idSubst_Tm sigma_Tm Eq_Tm s2)
+  | rfl _ s0 =>
+      congr_rfl (idSubst_Tm sigma_Tm Eq_Tm s0)
+  | jcase _ s0 s1 s2 =>
+      congr_jcase (idSubst_Tm sigma_Tm Eq_Tm s0) (idSubst_Tm sigma_Tm Eq_Tm s1) (idSubst_Tm sigma_Tm Eq_Tm s2)
   end.
 
 Lemma upExtRen_Tm_Tm {m : nat} {n : nat} (xi : fin m -> fin n)
@@ -229,6 +279,12 @@ Fixpoint extRen_Tm {m_Tm : nat} {n_Tm : nat} (xi_Tm : fin m_Tm -> fin n_Tm)
            (upExtRen_Tm_Tm _ _ Eq_Tm) s1)
   | tuniv _ => congr_tuniv
   | fix_ _ s0 => congr_fix_ (extRen_Tm xi_Tm zeta_Tm Eq_Tm s0)
+  | tid _ s0 s1 s2 =>
+      congr_tid (extRen_Tm xi_Tm zeta_Tm Eq_Tm s0) (extRen_Tm xi_Tm zeta_Tm Eq_Tm s1) (extRen_Tm xi_Tm zeta_Tm Eq_Tm s2)
+  | rfl _ s0 =>
+      congr_rfl (extRen_Tm xi_Tm zeta_Tm Eq_Tm s0)
+  | jcase _ s0 s1 s2 =>
+      congr_jcase (extRen_Tm xi_Tm zeta_Tm Eq_Tm s0) (extRen_Tm xi_Tm zeta_Tm Eq_Tm s1) (extRen_Tm xi_Tm zeta_Tm Eq_Tm s2)
   end.
 
 Lemma upExt_Tm_Tm {m : nat} {n_Tm : nat} (sigma : fin m -> Tm n_Tm)
@@ -278,6 +334,12 @@ Fixpoint ext_Tm {m_Tm : nat} {n_Tm : nat} (sigma_Tm : fin m_Tm -> Tm n_Tm)
            s1)
   | tuniv _ => congr_tuniv
   | fix_ _ s0 => congr_fix_ (ext_Tm sigma_Tm tau_Tm Eq_Tm s0)
+  | tid _ s0 s1 s2 =>
+      congr_tid (ext_Tm sigma_Tm tau_Tm Eq_Tm s0) (ext_Tm sigma_Tm tau_Tm Eq_Tm s1) (ext_Tm sigma_Tm tau_Tm Eq_Tm s2)
+  | rfl _ s0 =>
+      congr_rfl (ext_Tm sigma_Tm tau_Tm Eq_Tm s0)
+  | jcase _ s0 s1 s2 =>
+      congr_jcase (ext_Tm sigma_Tm tau_Tm Eq_Tm s0) (ext_Tm sigma_Tm tau_Tm Eq_Tm s1) (ext_Tm sigma_Tm tau_Tm Eq_Tm s2)
   end.
 
 Lemma up_ren_ren_Tm_Tm {k : nat} {l : nat} {m : nat} (xi : fin k -> fin l)
@@ -327,6 +389,12 @@ ren_Tm zeta_Tm (ren_Tm xi_Tm s) = ren_Tm rho_Tm s :=
            (upRen_Tm_Tm rho_Tm) (up_ren_ren _ _ _ Eq_Tm) s1)
   | tuniv _ => congr_tuniv
   | fix_ _ s0 => congr_fix_ (compRenRen_Tm xi_Tm zeta_Tm rho_Tm Eq_Tm s0)
+  | tid _ s0 s1 s2 =>
+      congr_tid (compRenRen_Tm xi_Tm zeta_Tm rho_Tm Eq_Tm s0) (compRenRen_Tm xi_Tm zeta_Tm rho_Tm Eq_Tm s1) (compRenRen_Tm xi_Tm zeta_Tm rho_Tm Eq_Tm s2)
+  | rfl _ s0 =>
+      congr_rfl (compRenRen_Tm xi_Tm zeta_Tm rho_Tm Eq_Tm s0)
+  | jcase _ s0 s1 s2 =>
+      congr_jcase (compRenRen_Tm xi_Tm zeta_Tm rho_Tm Eq_Tm s0) (compRenRen_Tm xi_Tm zeta_Tm rho_Tm Eq_Tm s1) (compRenRen_Tm xi_Tm zeta_Tm rho_Tm Eq_Tm s2)
   end.
 
 Lemma up_ren_subst_Tm_Tm {k : nat} {l : nat} {m_Tm : nat}
@@ -385,6 +453,12 @@ subst_Tm tau_Tm (ren_Tm xi_Tm s) = subst_Tm theta_Tm s :=
            (up_Tm_Tm theta_Tm) (up_ren_subst_Tm_Tm _ _ _ Eq_Tm) s1)
   | tuniv _ => congr_tuniv
   | fix_ _ s0 => congr_fix_ (compRenSubst_Tm xi_Tm tau_Tm theta_Tm Eq_Tm s0)
+  | tid _ s0 s1 s2 =>
+      congr_tid (compRenSubst_Tm xi_Tm tau_Tm theta_Tm Eq_Tm s0) (compRenSubst_Tm xi_Tm tau_Tm theta_Tm Eq_Tm s1) (compRenSubst_Tm xi_Tm tau_Tm theta_Tm Eq_Tm s2)
+  | rfl _ s0 =>
+      congr_rfl (compRenSubst_Tm xi_Tm tau_Tm theta_Tm Eq_Tm s0)
+  | jcase _ s0 s1 s2 =>
+      congr_jcase (compRenSubst_Tm xi_Tm tau_Tm theta_Tm Eq_Tm s0) (compRenSubst_Tm xi_Tm tau_Tm theta_Tm Eq_Tm s1) (compRenSubst_Tm xi_Tm tau_Tm theta_Tm Eq_Tm s2)
   end.
 
 Lemma up_subst_ren_Tm_Tm {k : nat} {l_Tm : nat} {m_Tm : nat}
@@ -466,6 +540,12 @@ ren_Tm zeta_Tm (subst_Tm sigma_Tm s) = subst_Tm theta_Tm s :=
   | tuniv _ => congr_tuniv
   | fix_ _ s0 =>
       congr_fix_ (compSubstRen_Tm sigma_Tm zeta_Tm theta_Tm Eq_Tm s0)
+  | tid _ s0 s1 s2 =>
+      congr_tid (compSubstRen_Tm sigma_Tm zeta_Tm theta_Tm Eq_Tm s0) (compSubstRen_Tm sigma_Tm zeta_Tm theta_Tm Eq_Tm s1) (compSubstRen_Tm sigma_Tm zeta_Tm theta_Tm Eq_Tm s2)
+  | rfl _ s0 =>
+      congr_rfl (compSubstRen_Tm sigma_Tm zeta_Tm theta_Tm Eq_Tm s0)
+  | jcase _ s0 s1 s2 =>
+      congr_jcase (compSubstRen_Tm sigma_Tm zeta_Tm theta_Tm Eq_Tm s0) (compSubstRen_Tm sigma_Tm zeta_Tm theta_Tm Eq_Tm s1) (compSubstRen_Tm sigma_Tm zeta_Tm theta_Tm Eq_Tm s2)
   end.
 
 Lemma up_subst_subst_Tm_Tm {k : nat} {l_Tm : nat} {m_Tm : nat}
@@ -548,6 +628,12 @@ subst_Tm tau_Tm (subst_Tm sigma_Tm s) = subst_Tm theta_Tm s :=
   | tuniv _ => congr_tuniv
   | fix_ _ s0 =>
       congr_fix_ (compSubstSubst_Tm sigma_Tm tau_Tm theta_Tm Eq_Tm s0)
+  | tid _ s0 s1 s2 =>
+      congr_tid (compSubstSubst_Tm sigma_Tm tau_Tm theta_Tm Eq_Tm s0) (compSubstSubst_Tm sigma_Tm tau_Tm theta_Tm Eq_Tm s1) (compSubstSubst_Tm sigma_Tm tau_Tm theta_Tm Eq_Tm s2)
+  | rfl _ s0 =>
+      congr_rfl (compSubstSubst_Tm sigma_Tm tau_Tm theta_Tm Eq_Tm s0)
+  | jcase _ s0 s1 s2 =>
+      congr_jcase (compSubstSubst_Tm sigma_Tm tau_Tm theta_Tm Eq_Tm s0) (compSubstSubst_Tm sigma_Tm tau_Tm theta_Tm Eq_Tm s1) (compSubstSubst_Tm sigma_Tm tau_Tm theta_Tm Eq_Tm s2)
   end.
 
 Lemma renRen_Tm {k_Tm : nat} {l_Tm : nat} {m_Tm : nat}
@@ -667,6 +753,12 @@ Fixpoint rinst_inst_Tm {m_Tm : nat} {n_Tm : nat}
            (rinstInst_up_Tm_Tm _ _ Eq_Tm) s1)
   | tuniv _ => congr_tuniv
   | fix_ _ s0 => congr_fix_ (rinst_inst_Tm xi_Tm sigma_Tm Eq_Tm s0)
+  | tid _ s0 s1 s2 =>
+      congr_tid (rinst_inst_Tm xi_Tm sigma_Tm Eq_Tm s0) (rinst_inst_Tm xi_Tm sigma_Tm Eq_Tm s1) (rinst_inst_Tm xi_Tm sigma_Tm Eq_Tm s2)
+  | rfl _ s0 =>
+      congr_rfl (rinst_inst_Tm xi_Tm sigma_Tm Eq_Tm s0)
+  | jcase _ s0 s1 s2 =>
+      congr_jcase (rinst_inst_Tm xi_Tm sigma_Tm Eq_Tm s0) (rinst_inst_Tm xi_Tm sigma_Tm Eq_Tm s1) (rinst_inst_Tm xi_Tm sigma_Tm Eq_Tm s2)
   end.
 
 Lemma rinstInst'_Tm {m_Tm : nat} {n_Tm : nat} (xi_Tm : fin m_Tm -> fin n_Tm)
@@ -871,6 +963,12 @@ Arguments ncase {n_Tm}.
 Arguments succ {n_Tm}.
 
 Arguments zero {n_Tm}.
+
+Arguments jcase {n_Tm}.
+
+Arguments rfl {n_Tm}.
+
+Arguments tid {n_Tm}.
 
 Arguments app {n_Tm}.
 
