theories/examples/finelt/validity.v
@@ -1,0 +1,49 @@
+From Stdlib Require Import Relations List Program
+     ssreflect ssrfun ssrbool.
+From Stdlib Require Import Classes.RelationClasses 
+  Classes.Morphisms Lia Arith.
+
+Set Implicit Arguments.
+Unset Strict Implicit.
+Unset Printing Implicit Defensive.
+
+Require Import smpl.Smpl.
+Require Import utils.all.
+
+Require Import syntax.syntax.
+Require Import syntax.typing.
+Require Import syntax.relations.
+Require Import syntax.reduction.
+
+From Stdlib Require Import ProofIrrelevance.
+Require Import finelt.utils.
+Require Import findom.
+Require Import types.
+Require Import selection.
+
+Require raw_validity.
+Module R := raw_validity.
+
+
+Import SyntaxNotations.
+Import SubstNotations.
+Import typing.Notations.
+
+Open Scope syntax_scope.
+Import Raw.
+
+Definition Val {n} (Γ : Ctx n) (M A : Tm n) {u a} (h: wt u a) : Prop := 
+  forall k, max (rk u) (rk a) < k -> R.Val k Γ M A h.
+Definition EqVal {n} (Γ : Ctx n) (M N A : Tm n) {u a} (h: wt u a) : Prop := 
+  forall k, max (rk u) (rk a) < k -> R.EqVal k Γ M N A h.
+Definition ValTy {n} (Γ : Ctx n) (M : Tm n) {u} (h: wt u tuniv) : Prop := 
+  forall k, max (rk u) 1 < k -> R.ValTy k Γ M h.
+Definition EqValTy {n} (Γ : Ctx n) (M N : Tm n) {u} (h: wt u tuniv) : Prop := 
+  forall k, max (rk u) 1 < k -> R.EqValTy k Γ M N h.
+
+Lemma EqVal_Val1 
+Lemma Val_EqVal
+Lemma Val_transport
+Lemma Val_transport_up
+
+
