theories/examples/syntax/declarative.v
@@ -1,0 +1,116 @@
+Require Import ssreflect.
+
+From Stdlib Require Export Logic.FunctionalExtensionality.
+From Stdlib Require Import Program.Equality.
+
+Require Export autosubst.core.
+Require Export autosubst.fintype.
+Require Import syntax.syntax.
+Require Import syntax.typing.
+
+Import SyntaxNotations.
+Import typing.Notations.
+Open Scope syntax_scope.
+
+Inductive typing : forall {n} (Γ : Ctx n), Tm n -> Tm n -> Prop := 
+
+  | t_var n (Γ : Ctx n) x : 
+    typing Γ (var x) (lookup x Γ)
+
+  | t_conv n (Γ : Ctx n) M A B : 
+    typing Γ M A -> 
+    conv Γ A B tuniv -> 
+    typing Γ M B
+
+  | t_abs n (Γ : Ctx n) A B N : 
+    typing Γ A tuniv ->
+    typing (ctx_extend Γ A) N B ->
+    typing Γ (abs A N) (tpi A B)
+
+  | t_app n (Γ : Ctx n) A B N M : 
+    typing Γ N (tpi A B) ->
+    typing Γ M A -> 
+    typing Γ (app N M) B[M..]
+
+  | t_nat n (Γ : Ctx n) : 
+    typing Γ tnat tuniv
+
+  | t_zero n (Γ : Ctx n) : 
+    typing Γ zero tnat 
+
+  | t_succ n (Γ : Ctx n) M : 
+    typing Γ M tnat ->
+    typing Γ (succ M) tnat 
+
+  | t_tpi n (Γ : Ctx n) A B : 
+    typing Γ A tuniv ->
+    typing (Γ ++ A) B tuniv -> 
+    typing Γ (tpi A B) tuniv
+
+  | t_univ n (Γ : Ctx n) : 
+    typing Γ tuniv tuniv
+
+with conv :forall {n} (Γ : Ctx n), Tm n -> Tm n -> Tm n -> Prop := 
+  | c_conv n (Γ : Ctx n) M N A B : 
+    conv Γ M N A -> 
+    conv Γ A B tuniv ->
+    conv Γ M N B
+
+  | c_refl n (Γ : Ctx n) M A : 
+    typing Γ M A ->
+    conv Γ M M A 
+
+  | c_sym n (Γ : Ctx n) M N A : 
+    conv Γ M N A -> 
+    conv Γ N M A
+
+  | c_trans n (Γ : Ctx n) M N P A  : 
+    conv Γ M N A -> 
+    conv Γ N P A -> 
+    conv Γ M P A
+
+  | c_app n (Γ : Ctx n) A B N N' M : 
+    conv Γ M M' (tpi A B) ->
+    conv Γ N N' A ->
+    conv Γ (app M N) (app M N') B[M..]
+
+  | c_beta n (Γ : Ctx n) A B M N :
+    typing Γ (abs A N) (tpi A B) -> 
+    typing Γ M A ->
+    conv Γ (app (abs A N) M) N[M..] B[M..]
+
+  | c_eta n (Γ : Ctx n) A B N N' :
+    typing Γ N (tpi A B) ->
+    typing Γ N' (tpi A B) ->
+    conv (Γ ++ A) 
+           (app N⟨↑⟩  (var var_zero))
+           (app N'⟨↑⟩ (var var_zero)) B ->
+    conv Γ N N' (tpi A B)
+
+  | c_succ n (Γ : Ctx n) M N :
+    conv Γ M N tnat ->
+    conv Γ (succ M) (succ N) tnat
+
+  | c_abs n (Γ : Ctx n) A A' B M M' :
+    typing Γ A tuniv ->
+    typing Γ A' tuniv ->
+    typing (ctx_extend Γ A) B tuniv ->
+    typing (ctx_extend Γ A) M B ->
+    typing (ctx_extend Γ A) M' B ->
+    conv Γ A A' tuniv ->
+    conv (ctx_extend Γ A) M M' B ->
+    conv Γ (abs A M) (abs A' M') (tpi A B)
+
+  | c_tpi n (Γ : Ctx n) A0 A1 B0 B1 :
+    typing Γ A0 tuniv ->
+    typing Γ A1 tuniv ->
+    typing (ctx_extend Γ A0) B0 tuniv ->
+    typing (ctx_extend Γ A1) B1 tuniv ->
+    conv Γ A0 A1 tuniv ->
+    conv (ctx_extend Γ A0) B0 B1 tuniv ->
+    conv Γ (tpi A0 B0) (tpi A1 B1) tuniv
+with ctx : forall {n}, Ctx n -> Prop :=
+  | c_empty : ctx ctx_empty
+  | c_cons n (Γ : Ctx n) A : ctx Γ -> 
+     typing Γ A tuniv -> 
+     ctx (ctx_extend Γ A).
